
Changing between polar and Cartesian coordinates

Starter

1. By possibly considering complex number equivalents, convert these points from polar form, (r, θ) to Cartesian form (x, y) :

(a) $\left(8, \frac{\pi}{6}\right)$ (b) $\left(6, -\frac{3\pi}{4}\right)$ (c) $\left(5, \frac{\pi}{2}\right)$

Working: (a) $\left(8, \frac{\pi}{6}\right) \equiv \left(8 \cos \frac{\pi}{6}, 8 \sin \frac{\pi}{6}\right) = (4\sqrt{3}, 4)$

(b) $\left(6, -\frac{3\pi}{4}\right) \equiv \left(6 \cos\left(-\frac{3\pi}{4}\right), 6 \sin\left(-\frac{3\pi}{4}\right)\right)$
 $= (-3\sqrt{2}, -3\sqrt{2})$

(c) $\left(5, \frac{\pi}{2}\right) \equiv \left(5 \cos \frac{\pi}{2}, 5 \sin \frac{\pi}{2}\right) = (0, 5)$

2. By possibly considering complex number equivalents, convert these points from Cartesian form (x, y) to polar form, (r, θ) :

(a) $(1, \sqrt{3})$ (b) $(-4, 4)$ (c) $(0, -6)$

Working: (a) $r = \sqrt{1^2 + (\sqrt{3})^2} = 2$

$$\theta = \tan^{-1} \frac{\sqrt{3}}{1} = \frac{\pi}{3}$$
$$(1, \sqrt{3}) \equiv \left(2, \frac{\pi}{3}\right)$$

(b) $r = \sqrt{(-4)^2 + 4^2} = \sqrt{32} = 4\sqrt{2}$

$(-4, 4)$ is in the 2nd quadrant so $\theta = \pi \tan^{-1} \frac{\sqrt{4}}{4} = \frac{3\pi}{4}$

$$(-4, 4) \equiv \left(4\sqrt{2}, \frac{3\pi}{4}\right)$$

(c) $r = 6$

The point is on the negative y -axis so $\theta = \frac{3\pi}{2}$

$$(0, -6) \equiv \left(6, \frac{3\pi}{2}\right)$$

E.g. 1 Convert $(x^2 + y^2)^2 = 4xy$ into polar form and state the family of curves from which it comes.

Working: $(x^2 + y^2)^2 = 4xy$

$$(x^2 + y^2)^2 = 4xy$$

$$(r^2)^2 = 4r \cos \theta \times r \sin \theta$$

$$r^4 = 2r^2 \sin 2\theta$$

$$r^2 = 2 \sin 2\theta$$

E.g. 2 Express these Cartesian equations in polar form:

(a) $y = x^2$

(b) $x \cos \alpha + y \sin \alpha = p$, where $p > 0$

Working: (a) $y = x^2$: $r \sin \theta = r^2 \cos^2 \theta$
 $r = \frac{\sin \theta}{\cos^2 \theta}$
 $r = \sec \theta \tan \theta$

(b) $x \cos \alpha + y \sin \alpha = p$: $r \cos \theta \cos \alpha + r \sin \theta \sin \alpha = p$
 $r(\cos \theta \cos \alpha + \sin \theta \sin \alpha) = p$
 $r \cos(\theta - \alpha) = p$

E.g. 3 Convert the polar equation $r = 2a \cos \theta$ to Cartesian form.

Working: $r = 2a \cos \theta$: $\sqrt{x^2 + y^2} = 2a \times \frac{x}{r}$
 $x^2 + y^2 = 2ax$

E.g. 4 Express these polar equations in Cartesian form:

(a) $r^2 = a^2 \sin 2\theta$

(b) $r = 2 \sin \theta$ for $0 \leq \theta < \pi$

Working: (a) $r^2 = a^2 \sin 2\theta$: $x^2 + y^2 = 2a^2 \cos \theta \sin \theta$
 $x^2 + y^2 = 2a^2 \times \frac{x}{r} \times \frac{y}{r}$
 $(x^2 + y^2)^2 = 2a^2 xy$

(b) $r = 2 \sin \theta$: $\sqrt{x^2 + y^2} = 2 \times \frac{y}{r}$
 $x^2 + y^2 = 2y$

Video: [Converting Cartesian to polar coordinates](#)

Video: [Converting polar to Cartesian coordinates](#)

Video: [Converting polar equations to Cartesian equations](#)

Video: [Converting Cartesian equations to polar equations](#)

[Solutions to Starter and E.g.s](#)

Exercise

p209 9C Qu 1i, 2i, 3i, 4i, 5-9